First-order proof mode tactics: `mlDestructEx`, `mlSpecialize`, `mlExists` (#324)
* Add lemma for mlIntro for universal quantifiers

* Finish first example

* Fix forall precedence

* mlRevertAll

* Add another forallintro-revert example

* Restructure tests

* Relax proof infos, restructure theorems

* Fix minor proof info bugs

* Create more FO. examples

* Fix FOL example

* mlExists, mlSpecialize

* Fix wrong quantifications: replaced them with openings

* mlDestructEx, and supporting tactics for free var inclusion

* Fix associativities, fix forall_subst inconsistencies, significantly simplify membership_elim

matching-logic/src/Pattern.v
@@ -140,8 +140,16 @@ Fixpoint size' (p : Pattern) : nat :=
     | patt_mu phi => free_svars phi
     end.
 
+  Definition free_evars_of_list l : EVarSet :=
+    union_list (map free_evars l).
 
-
+  Lemma free_evars_of_list_foldr :
+    forall l g,
+      free_evars (foldr patt_imp g l) =
+      free_evars g ∪ free_evars_of_list l.
+  Proof.
+    induction l; intro g; set_solver.
+  Qed.
 
   (* for bound set variables *)
   Fixpoint no_negative_occurrence_db_b (dbi : db_index) (ϕ : Pattern) : bool :=
